
基本公式
            重要极限一：$\lim_{x\rightarrow 0}\frac{sinx}{x}=1$
            重要极限二：$\lim_{x\rightarrow \infty}(1+\frac{1}{x})^x=e$，$\lim_{x\rightarrow 0}(1+x)^\frac{1}{x}=e$
            二项式定理
            对数公式1：$\LARGE a^x=e^{lna^x}=e^{xlna}$
            对数公式2：$\LARGE lne=1$
求导公式
            导数定义式
            1.$C'=0$
            2.$x'=1$
            3.$(x^n)' =nx^{n-1}$
            4.$(a^x)'=a^x\cdot lna$
            5.$(e^x)'=e^x$
            6.$(lnx)'=\frac{1}{x}$
            7.$(log_ax)'=\frac{1}{x\cdot lna}$
            8.$(sinx)'=cosx$
            9.$(cosx)'=-sinx$
            10.$(tanx)'=sec^2x$
            11.$(cotx)'=-csc^2x$
            12.$(secx)'=tanx\cdot secx$
            13.$(cscx)'=-cotx\cdot cscx$
            14.$(arcsinx)'=\frac{1}{\sqrt{1-x^2}}$
            15.$(arccosx)'=-\frac{1}{\sqrt{1-x^2}}$
            16.$(arctanx)'=\frac{1}{1+x^2}$
            17.$(arccotx)'=-\frac{1}{1+x^2}$
积分公式
            积分定义式：$\int f(x)dx=F(x)+C$,$\int dF(x)=F(x)+C$
            1.$\int kf(x)dx=kx+C$
            2.$\int x^ndx=\frac{x^{n-1}}{n-1}+C$
            4.$\int a^xdx=\frac{a^x}{lna}+C$
            4.$\int e^xdx=e^x+C$
            5.$\int \frac{1}{x}dx=ln|x|+C$
            6.$\int lnxdx=xlnx-x+C$
            7.$\int cosxdx=sinx+C$
            8.$\int sinxdx=-cosx+C$
            9.$\int sec^2xdx=tanx+C$
            10.$\int csc^2xdx=-cotx+C$
            11.$\int secx\cdot tanxdx=secx+C$
            12.$\int cscx\cdot cotxdx=-cscx+C$
            13.$\int \frac{1}{\sqrt{1-x^2}}dx=arcsin+C$
            14.$\int \frac{1}{1+x^2}dx=arctanx+C$
            15.$\int \frac{1}{\sqrt{a^2-x^2}}dx=arcsin\frac{x}{a}+C$
            16.$\int \frac{1}{a^2+x^2}dx=\frac{1}{a}arctan\frac{x}{a}+C$
            17.$\int tanxdx=-ln|cosx|+C$
            18.$\int cotxdx=ln|sinx|+C$
            19.$\int cscxdx=ln|tan\frac{x}{2}|+C=ln|cscx-cotx|+C$
            20.$\int secxdx=ln|secx+tanx|+C$
            21.$\int \frac{1}{x^2-a^2}dx=\frac{1}{2a} ln\Big|\frac{x-a}{x+a}\Big| +C$
            22.$\int\frac{1}{\sqrt{x^2\pm a^2}}dx=ln|x+\sqrt{x^2\pm a^2}|+C$

# 基本公式
#### 重要极限一：$\lim_{x\rightarrow 0}\frac{sinx}{x}=1$
$$
\begin{align}
\text{when $x\rightarrow0$, }&sinx\le x\le tanx\\
&1\le \frac{x}{sinx}\le \frac{tanx}{sinx}\\
&1\le \frac{x}{sinx}\le \frac{1}{cosx}\\
&cosx\le \frac{sinx}{x}\le 1\\
&\lim_{x\rightarrow 0}cosx=1\\
&\lim_{x\rightarrow 0}1=1\\
\because &\lim_{x\rightarrow 0}cosx\le \lim_{x\rightarrow 0}\frac{sinx}{x}\le \lim_{x\rightarrow 0}1\\
\therefore &1\le \lim_{x\rightarrow 0}\frac{sinx}{x}\le 1\\
\therefore&\lim_{x\rightarrow 0}\frac{sinx}{x}=1
\end{align}
$$
#### 重要极限二：$\lim_{x\rightarrow \infty}(1+\frac{1}{x})^x=e$，$\lim_{x\rightarrow 0}(1+x)^\frac{1}{x}=e$
$$

$$
#### 二项式定理
$$
(a+b)^n=\sum_{i=0}^{n} C _n^i a^{n-i}b^i\tag{A}
$$
$$
C_n^i=\frac{n!}{i!(n-i)!}\tag{B}
$$
#### 对数公式1：$\LARGE a^x=e^{lna^x}=e^{xlna}$

$$
\begin{align}
e^{lna^x}&=e^{log_ea^x} \\
&=a^x\tag{对数F.b}\\
e^{lna^x}&=e^{log_ea^x} \\
&=e^{xlog_ea}\tag{对数F.e} \\
&=e^{xlna}
\end{align}
$$
#### 对数公式2：$\LARGE lne=1$
$$
lne=log_ee\Longrightarrow e^1=e \Longrightarrow lne=1
$$
# 求导公式

#### 导数定义式
$$
\begin{align}
f'(x)&=\lim_{\Delta x\rightarrow0}\frac{f(x+\Delta x)-f(x)}{\Delta x} \\
\\&or \\
f'(x)&=\lim_{x_0\rightarrow\infty}\frac{f(x+x_0)-f(x)}{x-x_0}
\end{align}
$$
#### 1.$C'=0$
$$
\begin{align} \\
f(x)&=C\\
f'(C)&=\lim_{\Delta x\rightarrow 0}\frac{f(x+0)-f(x)}{0} \\
f'(C)&=\lim_{\Delta x\rightarrow 0}\frac{C-C}{0}=0
\end{align}
$$
#### 2.$x'=1$
$$
\begin{align} 
f(x)&=x\\
f'(x)&=\lim_{\Delta x\rightarrow 0}\frac{f(x+\Delta x)-f(x)}{\Delta x} \\
&=\lim_{\Delta x\rightarrow 0}\frac{x+\Delta x-x}{\Delta x} \\
&=\frac{\Delta x}{\Delta x}=1
\end{align}
$$
#### 3.$(x^n)' =nx^{n-1}$
$$
\begin{align}
f(x)&=x^n \\
f'(x^n)&=\lim_{\Delta x\rightarrow 0}\frac{(x+\Delta x)^n-x^n}{\Delta x} \\
&=\lim_{\Delta x\rightarrow 0}\frac{(
x^n +nx^{n-1}\Delta x+\cdots+nx\Delta x^{n-1}+\Delta x^n
)-x^n}{\Delta x} \tag{二项式} \\
&=\lim_{\Delta x\rightarrow 0}\frac{
 nx^{n-1}\Delta x+\cdots+nx\Delta x^{n-1}+\Delta x^n}{\Delta x}\tag{抵消$x^n$}\\
 &=\lim_{\Delta x\rightarrow 0}nx^{n-1}+\cdots+nx\Delta x^{n-2}+\Delta x^{n-1}\tag{全除$\Delta x$}\\
 &=\lim_{\Delta x\rightarrow 0}nx^{n-1}\tag{$\Delta x$项是0}\\
 &=nx^{n-1}
\end{align}
$$

#### 4.$(a^x)'=a^x\cdot lna$
$$
\begin{align}
\because f(x)&=a^x \\
a^x&=e^{xlna} \tag{对数公式1 }\\
\therefore (a^x)'&=(e^{xlna})' \\
&=e^{xlna}\cdot [x'\cdot lna+x\cdot (lna)']\tag{$lna$是常数}\\
&=e^{xlna}\cdot lna\\
&=a^x\cdot lna
\end{align}
$$
$$\LARGE\downarrow\uparrow推导出$$
#### 5.$(e^x)'=e^x$
$$
\begin{align}
f(x)&=e^x \\
(e^x)'&=\lim_{\Delta x\rightarrow 0}\frac{e^{(x+\Delta x)}-e^x}{\Delta x}\\
&=\lim_{\Delta x\rightarrow 0}\frac{e^{x}\cdot e^{\Delta x}-e^x}{\Delta x}\\
&=\lim_{\Delta x\rightarrow 0}\frac{e^{x}(e^{\Delta x}-1)}{\Delta x} \\
&=e^{x}\cdot \lim_{\Delta x\rightarrow 0}\frac{e^{\Delta x}-1}{\Delta x} \\
\text{令$u=e^{\Delta x}-1$, }&\text{则$e^{\Delta x}=1+n ,\Delta x=ln(1+n)$}\\
&=e^{x}\cdot \lim_{u\rightarrow 0}\frac{u}{ln(1+u)} \\
&=e^{x}\cdot \lim_{u\rightarrow 0}\frac{1}{\frac{1}{u}ln(1+u)} \tag{上下同除u}\\
&=e^{x}\cdot \lim_{u\rightarrow 0}\frac{1}{ln(1+u)^\frac{1}{u}} \\
&=e^{x}\cdot \lim_{u\rightarrow 0}\frac{1}{lne} =e^x\cdot1=e^x\\
\end{align}
$$
or
$$
\begin{align}
f(x)&=e^x \\
(e^x)'&=e^x\cdot lne \\
&=e^x\cdot1=e^x\tag{对数公式2}
\end{align}
$$
#### 6.$(lnx)'=\frac{1}{x}$
$$
\begin{align}
f(x)&=lnx\\
(lnx)'&=\lim_{\Delta x\rightarrow 0}\frac{ln(x+\Delta x)-lnx}{\Delta x} \\
&=\lim_{\Delta x\rightarrow 0}\frac{1}{\Delta x} \cdot ln(\frac{x+\Delta x}{x}) \\
&=\lim_{\Delta x\rightarrow 0}\frac{1}{\Delta x} \cdot ln(1+\frac{\Delta x}{x}) \\
&=\lim_{\Delta x\rightarrow 0} ln(1+\frac{\Delta x}{x}) ^{\frac{1}{\Delta x}} \\
&=ln\Big[\lim_{\Delta x\rightarrow 0} (1+\frac{\Delta x}{x}) ^{\frac{1}{\Delta x}}\Big] \\
&=ln\Big[\lim_{\Delta x\rightarrow 0} (1+\frac{\Delta x}{x}) ^{\frac{x}{\Delta x}\cdot\frac{1}{x}}\Big]\tag{重要极限} \\
&=lne^{\frac{1}{x}}=\frac{1}{x}
\end{align}
$$
$$
\LARGE\downarrow推导出
$$
#### 7.$(log_ax)'=\frac{1}{x\cdot lna}$
$$
\begin{align}
f(x)&=log_ax \\
log_ax&=\frac{lnx}{lna}\tag{换底公式} \\
(log_ax)'&=(\frac{1}{lna}\cdot lnx)'\tag{$lna$是常数} \\
&=\frac{1}{lna}\cdot \frac{1}{x}=\frac{1}{xlna}
\end{align}
$$
#### 8.$(sinx)'=cosx$
$$
\begin{align}
f(x)&=sinx \\
(sinx)'&=\lim_{\Delta x\rightarrow0}\frac{sin(x+\Delta x)-sinx}{\Delta x} \\
&=\lim_{\Delta x\rightarrow0}\frac{sinx\cdot cos\Delta x+cosx\cdot sin\Delta x-sinx}{\Delta x} \tag{倍角}\\
&=\lim_{\Delta x\rightarrow0}\frac{sinx\cdot (cos\Delta x-1)+cosx\cdot sin\Delta x}{\Delta x} \\
&=\lim_{\Delta x\rightarrow0}\frac{sinx\cdot (cos\Delta x-1)}{\Delta x}+\frac{cosx\cdot sin\Delta x}{\Delta x} \\
&=\lim_{\Delta x\rightarrow0}\frac{sinx\cdot (-\frac{1}{2}\Delta x^2)}{\Delta x}+\frac{cosx\cdot \Delta x}{\Delta x}\tag{等价} \\
&=cosx
\end{align}
$$
#### 9.$(cosx)'=-sinx$
$$
\begin{align}
f(x)&=cosx \\
(cosx)'&=\lim_{\Delta x\rightarrow0}\frac{cos(x+\Delta x)-cosx}{\Delta x} \\
&=\lim_{\Delta x\rightarrow0}\frac{cosx\cdot cos\Delta x-sinx\cdot sin\Delta x-cosx}{\Delta x} \tag{倍角}\\
&=\lim_{\Delta x\rightarrow0}\frac{cosx\cdot (cos\Delta x-1)-sinx\cdot sin\Delta x}{\Delta x} \\
&=\lim_{\Delta x\rightarrow0}\frac{cosx\cdot (-\frac{1}{2}\Delta x^2)-sinx\cdot \Delta x}{\Delta x}\tag{等价}  \\
&=-sinx
\end{align}
$$
#### 10.$(tanx)'=sec^2x$
$$
\begin{align}
f(x)&=tanx \\
(tanx)'&=(\frac{sinx}{cosx})' \\
&=\frac{cosx\cdot cosx+sinx\cdot sinx}{cos^2x}\tag{四则} \\
&=\frac{cos^2x+sin^2x}{cos^2x} \tag{同角}\\
&=\frac{1}{cos^2x} \\
&=\frac{1}{cos^2x}=sec^2x
\end{align}
$$
#### 11.$(cotx)'=-csc^2x$
$$
\begin{align}
f(x)&=cot \\
(cot)'&=(\frac{cosx}{sinx})' \\
&=\frac{-sinx\cdot sinx-cosx\cdot cosx}{sin^2x}\tag{四则} \\
&=\frac{-cos^2x-sin^2x}{sin^2x} \\
&=\frac{-(cos^2x+sin^2x)}{sin^2x} \tag{同角}\\
&=\frac{-1}{sin^2x}=-csc^2x
\end{align}
$$
#### 12.$(secx)'=tanx\cdot secx$
$$
\begin{align}
f(x)&=secx \\
(secx)'&=(\frac{1}{cosx})' \\ 
&=\frac{0\cdot cosx+1\cdot  sinx}{cos^2x}\tag{四则} \\
&=\frac{sinx}{cos^2x} \\
&=\frac{sinx}{cosx}\cdot\frac{1}{cosx}=tanx\cdot secx
\end{align}
$$
#### 13.$(cscx)'=-cotx\cdot cscx$
$$
\begin{align}
f(x)&=cscx \\
(cscx)'&=(\frac{1}{sinx})' \\ 
&=\frac{0\cdot sinx-1\cdot  cosx}{sin^2x}\tag{四则} \\
&=\frac{-cosx}{sin^2x} \\
&=\frac{-cosx}{sinx}\cdot\frac{1}{sinx}=-cotx\cdot cscx
\end{align}
$$
#### 14.$(arcsinx)'=\frac{1}{\sqrt{1-x^2}}$
$$
\begin{align}
f(x)&=arcsinx \\
\because y=&arcsinx~,~x=siny~,~x'=cosy  \\
y'=&\frac{dy}{dx}~,~x'=\frac{dx}{dy}\\ 
\therefore y'=&\frac{1}{x'}\\
(arcsinx)'&=\frac{1}{cosy}\\ 
&=\frac{1}{\sqrt{1-sin^2y}} \tag{同角}\\
&=\frac{1}{\sqrt{1-x^2}}\tag{$x=siny换回$}\\
\end{align}
$$
#### 15.$(arccosx)'=-\frac{1}{\sqrt{1-x^2}}$
$$
\begin{align}
f(x)&=arccosx \\
\because y=&arccosx~,~x=cosy~,~x'=-siny  \\
y'=&\frac{dy}{dx}~,~x'=\frac{dx}{dy}\\ 
\therefore y'=&\frac{1}{x'}\\
(arcsinx)'&=-\frac{1}{siny}\\ 
&=-\frac{1}{\sqrt{1-cos^2y}} \tag{同角}\\
&=-\frac{1}{\sqrt{1-x^2}}\tag{$x=cosy换回$}\\
\end{align}
$$
#### 16.$(arctanx)'=\frac{1}{1+x^2}$
$$
\begin{align}
f(x)&=arctanx \\
\because y=&arctanx~,~x=tany~,~x'=sec^2y  \\
y'=&\frac{dy}{dx}~,~x'=\frac{dx}{dy}\\ 
\therefore y'=&\frac{1}{x'}\\
(arctanx)'&=\frac{1}{sec^2y}\\ 
&=\frac{1}{1+tan^2y} \tag{同角}\\
&=\frac{1}{1+x^2}\tag{$x=tany换回$}\\
\end{align}
$$
#### 17.$(arccotx)'=-\frac{1}{1+x^2}$
$$
\begin{align}
f(x)&=arccotx \\
\because y=&arccotx~,~x=coty~,~x'=-csc^2y  \\
y'=&\frac{dy}{dx}~,~x'=\frac{dx}{dy}\\ 
\therefore y'=&\frac{1}{x'}\\
(arccotx)'&=-\frac{1}{csc^2y}\\ 
&=-\frac{1}{1+cot^2y} \tag{同角}\\
&=-\frac{1}{1+x^2}\tag{$x=tany换回$}\\
\end{align}
$$

# 积分公式

#### 积分定义式：$\int f(x)dx=F(x)+C$,$\int dF(x)=F(x)+C$
$$
\LARGE\downarrow推导出
$$
#### 1.$\int kf(x)dx=kx+C$
$$
\begin{align}
\int kf(x)dx &=k\int f(x)dx\\
&=kx+C
\end{align}
$$
#### 2.$\int x^ndx=\frac{x^{n-1}}{n-1}+C$
$$
\begin{align}
\because (x^{n+1})'&=(n+1)x^n\tag{凑微分法} \\
\therefore (n+1)x^n&=\frac{d}{dy}x^{n+1} \\
\int(n+1)x^n dx&=\int \frac{d}{dy}x^{n+1} \\
\int x^n dx&=\frac{1}{(n+1)}\int \frac{d}{dy}x^{n+1}  \\
&=\int \frac{d}{dy} \frac{x^{n+1}}{(n+1)} \\
&=\frac{x^{n+1}}{(n+1)}+C\tag{定义式}
\end{align}
$$
#### 4.$\int a^xdx=\frac{a^x}{lna}+C$
$$
\begin{align}
\because (a^x)'&=a^xlna\tag{凑微分法} \\
\therefore a^xlna&=\frac{d}{dy}a^x \\
\int a^xlna dx&=\int \frac{d}{dy}a^x \\
\int a^x dx&=\frac{1}{lna}\int \frac{d}{dy}a^x  \\
&=\int \frac{d}{dy} \frac{a^x}{lna} \\
&=\frac{a^x}{lna}+C\tag{定义式}
\end{align}
$$
$$
\LARGE\downarrow推导出
$$
#### 4.$\int e^xdx=e^x+C$
$$
\begin{align}
&=\frac{e^x}{lne}+C \\
&=e^x+C
\end{align}
$$
#### 5.$\int \frac{1}{x}dx=ln|x|+C$
当$x>0时，(lnx)'=\frac{1}{x}$
$$
\int\frac{1}{x}dx=\int dlnx=lnx+C
$$
当$x<0时，(ln(-x))'=\frac{1}{-x}\cdot(-1)=\frac{1}{x}$
$$
\int\frac{1}{x}dx=\int dln(-x)=ln(-x)+C
$$
$$
\therefore \int\frac{1}{x}dx=ln|x|+C
$$
#### 6.$\int lnxdx=xlnx-x+C$
$$
\begin{align}
\int lnxdx&=lnx\cdot x-\int xdlnx\tag{分部积分} \\
&=lnx\cdot x-\int x\frac{1}{x}dx \\
&=lnx\cdot x-x+C \\
\end{align}
$$
#### 7.$\int cosxdx=sinx+C$
$$
凑微分法\tag{refer 积分2}
$$
#### 8.$\int sinxdx=-cosx+C$
$$
凑微分法\tag{refer 积分2}
$$
#### 9.$\int sec^2xdx=tanx+C$
$$
凑微分法\tag{refer 积分2}
$$
#### 10.$\int csc^2xdx=-cotx+C$
$$
凑微分法\tag{refer 积分2}
$$
#### 11.$\int secx\cdot tanxdx=secx+C$
$$
凑微分法\tag{refer 积分2}
$$
#### 12.$\int cscx\cdot cotxdx=-cscx+C$
$$
凑微分法\tag{refer 积分2}
$$
#### 13.$\int \frac{1}{\sqrt{1-x^2}}dx=arcsin+C$
$$
凑微分法\tag{refer 积分2}
$$
#### 14.$\int \frac{1}{1+x^2}dx=arctanx+C$
$$
凑微分法\tag{refer 积分2}
$$
#### 15.$\int \frac{1}{\sqrt{a^2-x^2}}dx=arcsin\frac{x}{a}+C$
$$
\begin{align}
\int \frac{1}{\sqrt{a^2-x^2}}dx &=\int \frac{1}{a\sqrt{1-(\frac{x}{a})^2}}dx \\
&=\int \frac{1}{a}\frac{1}{\sqrt{1-(\frac{x}{a})^2}}dx \\
&=\int \frac{1}{\sqrt{1-(\frac{x}{a})^2}}d(\frac{x}{a})\\
&=arcsin\frac{x}{a}+C 
\end{align}
$$
#### 16.$\int \frac{1}{a^2+x^2}dx=\frac{1}{a}arctan\frac{x}{a}+C$
$$
\begin{align}
\int \frac{1}{a^2+x^2}dx 
&=\int \frac{1}{a^2}\frac{1}{1+(\frac{x}{a})^2}dx  \\
&=\frac{1}{a}\int \frac{1}{1+(\frac{x}{a})^2}d(\frac{x}{a})  \\
&=\frac{1}{a}arctan\frac{x}{a}+C 
\end{align}
$$
#### 17.$\int tanxdx=-ln|cosx|+C$
$$
\begin{align}
\int tanxdx&=\int\frac{sinx}{cosx}dx \\
&=\int\frac{1}{cosx}d(-cos) \\
&=-\int\frac{1}{cosx}d(cos) \\
&=-ln|cosx|+C
\end{align}
$$
#### 18.$\int cotxdx=ln|sinx|+C$
$$
\begin{align}
\int cotxdx&=\int\frac{cosx}{sinx}dx \\
&=\int\frac{1}{sinx}d(sinx) \\
&=ln|sinx|+C
\end{align}
$$
#### 19.$\int cscxdx=ln|tan\frac{x}{2}|+C=ln|cscx-cotx|+C$
$$
\begin{align}
\int cscxdx&=\int \frac{1}{sinx}dx \\
&=\int\frac{1}{2sin\frac{x}{2}cos\frac{x}{2}}dx \tag{refer 倍角11}\\
&=\int\frac{1}{sin\frac{x}{2}cos\frac{x}{2}}d(\frac{x}{2}) \\
&=\int\frac{1}{\frac{sin\frac{x}{2}}{cos\frac{x}{2}}cos^2\frac{x}{2}}d(\frac{x}{2})  \\
&=\int\frac{1}{tan\frac{x}{2}}d(tan\frac{x}{2})\tag{refer 积分9} \\
&=ln|tan\frac{x}{2}|+C\tag{conclusion 1} \\
\because tan\frac{x}{2}&=\frac{sin\frac{x}{2}}{cos\frac{x}{2}} \\
&=\frac{sin\frac{x}{2}}{cos\frac{x}{2}} \cdot\frac{2sin\frac{x}{2}}{2sin\frac{x}{2}} \\
&=\frac{2sin^2\frac{x}{2}}{2sin\frac{x}{2}cos\frac{x}{2}} \\
&=\frac{1-cosx}{sinx} \tag{refer 半角13\&倍角11} \\
&=\frac{1}{sinx}-\frac{cosx}{sinx} \\
&=cscx-cotx \\
\therefore \int cscxdx&=ln|cscx-cotx|+C\tag{conclusion 2}
\end{align}
$$
$$
\LARGE\downarrow推导出
$$
#### 20.$\int secxdx=ln|secx+tanx|+C$
$$
\begin{align} 
\int secxdx&=\int csc(x+\frac{\pi}{2})d(x+\frac{\pi}{2}) \tag{refer 三角III}\\
&=ln|csc(x+\frac{\pi}{2})-cot(x+\frac{\pi}{2})|+C \\
&=ln|secx+tanx|+C \tag{诱导公式}\\
\end{align}
$$
#### 21.$\int \frac{1}{x^2-a^2}dx=\frac{1}{2a} ln\Big|\frac{x-a}{x+a}\Big| +C$
$$
\begin{align}\because \frac{1}{x^2-a^2}&=\frac{A}{x-a}+\frac{B}{x+a}  \\
&=\frac{A(x+a)+B(x-a)}{(x-a)(x+a)}\\
&=\frac{Ax+Aa+Bx-Ba}{(x-a)(x+a)} \\
&=\frac{(A+B)x+(A-B)a}{(x-a)(x+a)} \\
\begin{cases}
A+B=0 \\
(A-B)a=1
\end{cases} 
&\Longrightarrow 
\begin{cases}
A+B=0 \\
A-B=\frac{1}{a}
\end{cases} 
\Longrightarrow 
\begin{cases}
A=\frac{1}{2a} \\
B=-\frac{1}{2a}
\end{cases}  \\
\therefore \int \frac{1}{x^2-a^2}dx &=\int(\frac{\frac{1}{2a} }{x-a}+\frac{-\frac{1}{2a} }{x+a})dx \\
&=\frac{1}{2a} \int(\frac{1}{x-a}-\frac{1}{x+a})dx \\
&=\frac{1}{2a} \Big[\int \frac{1}{x-a}d(x-a)-\int\frac{1}{x+a} d(x+a)\Big] \\
&=\frac{1}{2a} \Big[ln|x-a|-ln|x+a|\Big] +C \\
&=\frac{1}{2a} ln\Big|\frac{x-a}{x+a}\Big| +C
\end{align}
$$
#### 22.$\int\frac{1}{\sqrt{x^2\pm a^2}}dx=ln|x+\sqrt{x^2\pm a^2}|+C$
proof 1
$$
\begin{align}
令~x&=a\cdot tant \\
\sqrt{x^2+a^2}&=\sqrt{a^2tan^2t+a^2} \\
&=\sqrt{a^2(tan^2t+1)} \\
&=\sqrt{a^2sec^2t} \\
&=a\cdot sect \\
dx&=d(a\cdot tant)=a\cdot sec^2tdt\tag{refer 求导 10} \\
tant&=\frac{x}{a}~,~sect=\frac{\sqrt{x^2+a^2}}{a}\\
\int \frac{1}{\sqrt{x^2+a^2}}dx &=\frac{a\cdot sec^2t}{a\cdot sect}dt \\
&=\int sectdt \\
&=ln|sect+tant|+C\tag{refer 积分 20} \\
&=ln|\frac{\sqrt{x^2+a^2}}{a}+\frac{x}{a}|+C \\
&=ln|\frac{\sqrt{x^2+a^2}+x}{a}|+C \\
&=ln|\sqrt{x^2+a^2}+x|-lna+C \\
&=ln|x+\sqrt{x^2+a^2}|+C\tag{conclusion 1}
\end{align}
$$
proof 2
$$
\begin{align}
令~x&=a\cdot sect  \\
\sqrt{x^2-a^2}&=\sqrt{a^2sec^2t-a^2} \\
&=\sqrt{a^2(sec^2t-1)} \\
&=\sqrt{a^2tan^2t} \\
&=a\cdot tant  \\
dx& = d(a\cdot sect)= a\cdot sect\cdot tant dt.\tag{refer 求导 12} \\
sect&=\frac{x}{a}~,~tant=\frac{\sqrt{x^2-a^2}}{a}\\
\int\frac{1}{\sqrt{x^2-a^2}}dx&=\int \frac{a\cdot sect\cdot tant}{a\cdot tant }dt \\
&=\int sectdt \tag{refer 积分 20}\\
&=ln|sect+tant|+C \\
&=ln|\frac{x}{a}+\frac{\sqrt{x^2-a^2}}{a}|+C  \\
&=ln|x+\sqrt{x^2-a^2}|-lna+C  \\
&=ln|x+\sqrt{x^2-a^2}|+C \tag{conclusion 2}
\end{align}
$$
synthesize 1 & 2
$$
\begin{align}
\int \frac{1}{\sqrt{x^2+a^2}}dx &=ln|x+\sqrt{x^2+a^2}|+C\\
\int\frac{1}{\sqrt{x^2-a^2}}dx&=ln|x+\sqrt{x^2-a^2}|+C  \\
\therefore \int\frac{1}{\sqrt{x^2\pm a^2}}dx&=ln|x+\sqrt{x^2\pm a^2}|+C
\end{align}
$$
